theories/cast_calc/cc.v
@@ -1,0 +1,17 @@
+From main.cast_calc Require
+  contexts definition labels types typing.
+From main.cast_calc.dynamics Require
+  lemmas std.
+
+Include contexts.
+Include definition.
+Include labels.
+Include types.
+Include typing.
+Include lemmas.
+Include std.
+
+(* aim of this file is to just gather all definitions related to cast calculus, such that I can easily refer to them; e.g. cc.fill_item *)
+
+(* use this file with  *)
+(* Require main.cc. *)
