theories/dyn_lang/dn.v
@@ -1,0 +1,10 @@
+From main.dyn_lang Require
+  casts contexts definition labels lemmas lib tactics.
+
+Include casts.
+Include contexts.
+Include definition.
+Include labels.
+Include lemmas.
+Include lib.
+Include tactics.
